checkpoint

src/Facade.v
@@ -1578,95 +1578,72 @@ Proof.
 Defined.
 Eval lazy in projT1 (micro_swap 0 1).
 
-Example micro_swap_args : sigT (fun p =>
-  forall a b, EXTRACT swap_prog a b {{ "a" ~> a; "b" ~> b; ∅ }} p {{ fun _ => ∅ }} // ∅).
+Example micro_swap_args : forall env, sigT (fun p =>
+  forall a b, EXTRACT swap_prog a b {{ "a" ~> a; "b" ~> b; ∅ }} p {{ fun _ => ∅ }} // env).
 Proof.
   intros.
   compile.
   intros.
   compile.
 Defined.
-Eval lazy in projT1 micro_swap_args.
+Eval lazy in projT1 (micro_swap_args ∅).
+
+Opaque swap_prog.
 
 Definition swap_env : Env :=
   ("swap" ->> {|
            ArgVars := ["a"; "b"];
-           RetVar := "r0"; Body := projT1 micro_swap_args;
+           RetVar := "r0"; Body := projT1 (micro_swap_args ∅);
            ret_not_in_args := ltac:(auto); args_no_dup := ltac:(auto)
          |}; ∅).
+
+Definition call_swap :=
+  swap_prog 0 1;;
+  Ret tt.
 
 Definition rot :=
   swap_prog 0 1;;
   swap_prog 1 2;;
   Ret tt.
 
-Ltac inv_exec_solve :=
-  intuition (subst; try discriminate; repeat find_inversion_safe;
-                                          repeat match_finds; simpl in *;
-                                          try solve [ exfalso; intuition eauto 10 ]; eauto 10).
+Axiom false : False.
+Tactic Notation "really_admit" := elim false.
 
-Example extract_rot :
-  sigT (fun p =>
-          EXTRACT rot {{ ∅ }} p {{ fun _ => ∅ }} // swap_env).
+Example swap_call : forall avar bvar, avar <> bvar -> sigT (fun p =>
+  forall a b, EXTRACT swap_prog a b {{ avar ~> a; bvar ~> b; ∅ }} p {{ fun _ => avar ~> a; bvar ~> b; ∅ }} // swap_env).
 Proof.
   eexists.
+  instantiate (p := Call "_" "swap" [avar; bvar]).
+  really_admit.
+Defined.
 
-  instantiate (p := ("c0" <~ Const 0; "c1" <~ Const 1; "c2" <~ Const 2;
-                    Call "_" "swap" ["c0"; "c1"]; Call "_" "swap" ["c1"; "c2"])%facade).
-  unfold ProgOk.
-  intros.
-  (*
-  Focus 2.
-  inv_exec_solve.
-  contradiction H1. destruct initial_state. eauto 10.
-  Focus 2.
-  inv_exec_solve.
-  invc H4.
-  invc H1.
+Definition swap_call_cor avar bvar abne := projT2 (@swap_call avar bvar abne).
+Hint Resolve swap_call_cor : extracted.
 
-
-Ltac inv_exec' :=
+Example extract_call_swap :
+  sigT (fun p =>
+          EXTRACT call_swap {{ ∅ }} p {{ fun _ => ∅ }} // swap_env).
+Proof.
+  compile.
+  eapply extract_equiv_prog; [ eapply bind_left_id | ].
+  compile.
   match goal with
-    | [ H : Step _ ?p _ |- _ ] =>
-      match p with
-        | (_, _, Body _) => fail 1
-        | _ => idtac
-      end;
-      invc H
-  | [ H : Exec _ ?p _ |- _ ] => (is_var p; fail 1) || invc H
-  | [ H : CrashStep _ |- _ ] => invc H
-  end; try discriminate.
-*)
-
-
-intuition.
-subst.
-find_eapply_lem_hyp ExecFinished_Steps.
-find_eapply_lem_hyp Steps_RunsTo.
-Ltac inv_runsto :=
-  match goal with
-    | [ H : RunsTo _ _ _ _ |- _ ] => invc H
-  end.
-inv_runsto.
-inv_runsto.
-inv_runsto.
-inv_runsto.
-invc H3.
-invc H4.
-invc H2.
-invc H5.
-unfold swap_env in *.
-maps.
-repeat find_inversion_safe.
-simpl in *.
-eapply RunsTo_Steps in H18.
-eapply Steps_ExecFinished in H18.
-pose proof micro_swap_args.
-unfold ProgOk in *.
-destruct X.
-(* need a weakening lemma which lets us know that micro_swap_args still works in an environment which is a superset *)
-Abort.
-
+      | [ |- EXTRACT ?goal {{ _ }} _ {{ _ }} // _ ] =>
+      eapply extract_equiv_prog; [
+        let arg := fresh "arg" in
+        set (arg := goal);
+        pattern 0 in arg; subst arg;
+        eapply bind_left_id | ] end.
+  compile.
+  eapply hoare_weaken_post.
+  shelve.
+  eauto with extracted.
+  Unshelve.
+  match_scopes.
+  maps.
+  congruence.
+Defined.
+Eval lazy in projT1 extract_call_swap.
 
 
 Definition swap2_prog :=
